CopyValue for tape_contains_v3

TM/Code/Copy.v
@@ -18,14 +18,15 @@ Generalizable All Variables.
 
 (* Don't simplify [skipn (S n) xs]; only, if the number and the lists are constructors *)
 Local Arguments skipn { A } !n !l.
-
+Local Arguments plus : simpl never.
+Local Arguments mult : simpl never.
 
 Section Copy.
 
   Variable sig : finType.
   Variable stop : sig -> bool.
 
-  Lemma CopySymbols_pair_correct tltr str1 x str2 :
+  Lemma CopySymbols_correct tltr str1 x str2 :
     (forall x, List.In x str1 -> stop x = false) ->
     (stop x = true) ->
     tape_local (fst tltr) = str1 ++ x :: str2 ->
@@ -46,8 +47,21 @@ Section Copy.
     - destruct t1; cbn in *; auto; now apply app_cons_not_nil in HEnc.
   Qed.
 
-  
-  Lemma CopySymbols_L_pair_correct tltr str1 x str2 :
+  Corollary CopySymbols_correct_midtape ls m rs x rs' t2 :
+    stop m = false ->
+    (forall x, List.In x rs -> stop x = false) ->
+    stop x = true ->
+    CopySymbols_Fun stop id (midtape ls m (rs ++ x :: rs'), t2) =
+    (midtape (rev rs ++ m :: ls) x rs',
+     midtape (rev rs ++ m :: left (t2)) x (skipn (S (|rs|)) (right t2))).
+  Proof.
+    intros HStopM HStopRs HStopX.
+    unshelve epose proof @CopySymbols_correct (midtape ls m (rs ++ x :: rs'), t2) (m::rs) x rs' _ _ _ as L; cbn in *; eauto.
+    - intros ? [->|?]; auto.
+    - now rewrite <- !app_assoc in L.
+  Qed.
+
+  Lemma CopySymbols_L_correct tltr str1 x str2 :
     (forall x, List.In x str1 -> stop x = false) ->
     (stop x = true) ->
     tape_local_l (fst tltr) = str1 ++ x :: str2 ->
@@ -68,7 +82,21 @@ Section Copy.
     - destruct t1; cbn in *; auto; now apply app_cons_not_nil in HEnc.
   Qed.
 
-  
+
+  Corollary CopySymbols_L_correct_midtape ls ls' m rs x t2 :
+    stop m = false ->
+    (forall x, List.In x ls -> stop x = false) ->
+    stop x = true ->
+    CopySymbols_L_Fun stop id (midtape (ls ++ x :: ls') m rs, t2) =
+    (midtape ls' x (rev ls ++ m :: rs),
+     midtape (skipn (S (|ls|)) (left t2)) x (rev ls ++ m :: right t2)).
+  Proof.
+    intros HStopM HStopRs HStopX.
+    unshelve epose proof @CopySymbols_L_correct (midtape (ls ++ x :: ls') m rs, t2) (m::ls) x ls' _ _ _ as L; cbn in *; eauto.
+    - intros ? [->|?]; auto.
+    - now rewrite <- !app_assoc in L.
+  Qed.
+
   Lemma MoveToSymbol_correct t str1 str2 x :
     (forall x, List.In x str1 -> stop x = false) ->
     (stop x = true) ->
@@ -103,7 +131,7 @@ Section Copy.
     { intros ? [->|?]; auto. }
     cbn in *. now rewrite <- app_assoc in L.
   Qed.
-    
+
   Corollary MoveToSymbol_L_correct t str1 str2 x :
     (forall x, List.In x str1 -> stop x = false) ->
     (stop x = true) ->
@@ -127,7 +155,7 @@ Section Copy.
     unshelve epose proof (@MoveToSymbol_L_correct (midtape (ls ++ x :: ls') m rs) (m::ls) ls' x _ HStopX eq_refl) as L.
     { intros ? [->|?]; auto. }
     cbn in *. now rewrite <- app_assoc in L.
-  Qed.    
+  Qed.
 
   Lemma MoveToSymbol_correct_toRight' (t : tape sig) x str :
     tape_local t = x :: str ->
@@ -152,7 +180,7 @@ Section Copy.
     pose proof @MoveToSymbol_correct_toRight' (midtape ls x rs) _ _ ltac:(cbn; eauto) as (L1&L2).
     rewrite L1, L2. cbn. simpl_list. cbn. simpl_list. cbn. auto.
   Qed.
-  
+
   Corollary MoveToSymbol_L_correct_toLeft ls (x : sig) rs :
     left (tape_move_right (MoveToSymbol_L_Fun (fun _ => false) (midtape ls x rs))) = nil /\
     tape_local (tape_move_right (MoveToSymbol_L_Fun (fun _ => false) (midtape ls x rs))) = rev ls ++ x :: rs.
@@ -193,7 +221,7 @@ Section Copy.
     cbn [length]. omega.
   Qed.
 
-  Lemma MoveToSymbol_TermTime_local_l t r1 sym r2 :
+  Lemma MoveToSymbol_L_TermTime_local t r1 sym r2 :
     tape_local_l t = r1 ++ sym :: r2 ->
     stop sym = true ->
     MoveToSymbol_L_TermTime stop t <= 4 + 4 * length r1.
@@ -207,15 +235,15 @@ Section Copy.
         eapply IHr1; eauto. cbn. now simpl_tape.
   Qed.
 
-  Corollary MoveToSymbol_TermTime_midtape_l ls ls' x m rs :
+  Corollary MoveToSymbol_L_TermTime_midtape ls ls' x m rs :
     stop x = true ->
     MoveToSymbol_L_TermTime stop (midtape (ls ++ x :: ls') m rs) <= 8 + 4 * length ls.
   Proof.
     intros.
-    rewrite MoveToSymbol_TermTime_local_l with (r1 := m::ls) (sym := x) (r2 := ls'); auto.
+    rewrite MoveToSymbol_L_TermTime_local with (r1 := m::ls) (sym := x) (r2 := ls'); auto.
     cbn [length]. omega.
   Qed.
-    
+
 
   Lemma MoveToSymbol_TermTime_dontstop t :
     MoveToSymbol_TermTime (fun x : sig => false) t <= 4 + 4 * (|tape_local t|).
@@ -236,8 +264,8 @@ Section Copy.
       + cbn -[plus mult] in *. omega.
     - omega.
   Qed.
-  
-  
+
+
 
   Lemma CopySymbols_TermTime_local t r1 sym r2 :
     tape_local t = r1 ++ sym :: r2 ->
@@ -253,7 +281,13 @@ Section Copy.
         eapply IHr1; eauto. cbn. now simpl_tape.
   Qed.
 
-  
+  Corollary CopySymbols_TermTime_midtape ls m rs x rs' :
+    stop x = true ->
+    CopySymbols_TermTime stop (midtape ls m (rs ++ x :: rs')) <= 16 + 8 * length rs.
+  Proof.
+    intros. erewrite CopySymbols_TermTime_local with (r1 := m :: rs); cbn -[plus mult]; eauto. omega.
+  Qed.
+
   Lemma CopySymbols_L_TermTime_local t r1 sym r2 :
     tape_local_l t = r1 ++ sym :: r2 ->
     stop sym = true ->
@@ -268,6 +302,12 @@ Section Copy.
         eapply IHr1; eauto. cbn. now simpl_tape.
   Qed.
 
+  Corollary CopySymbols_L_TermTime_midtape ls x ls' m rs :
+    stop x = true ->
+    CopySymbols_L_TermTime stop (midtape (ls ++ x :: ls') m rs) <= 16 + 8 * length ls.
+  Proof.
+    intros. erewrite CopySymbols_L_TermTime_local with (r1 := m :: ls); cbn -[plus mult]; eauto. omega.
+  Qed.
 
 End Copy.
 
@@ -280,7 +320,7 @@ Section Move.
 
   Definition isStop  (s: sig^+) := match s with inl STOP => true | _ => false end.
   Definition isStart (s: sig^+) := match s with inl START => true | _ => false end.
-  
+
   (* Note, that [encode] maps implicitely here *)
   Lemma stop_not_in (x : X) (s : (sig^+)) :
     List.In s (encode x) -> isStop s = false.
@@ -315,7 +355,7 @@ Section Move.
       - apply stop_not_in.
     }
   Qed.
-  
+
   Lemma MoveLeft_WRealise : MoveLeft ⊫ MoveLeft_Rel.
   Proof.
     eapply WRealise_monotone.
@@ -326,7 +366,7 @@ Section Move.
       destruct HEncX as (r1&->).
       erewrite MoveToSymbol_L_correct_midtape; eauto.
       - repeat econstructor. now rewrite <- map_rev, rev_involutive.
-      - intros ? (?&<-&? % in_rev) % in_map_iff. reflexivity.
+      - intros ? (?&<-&?) % in_map_iff. reflexivity.
     }
   Qed.
 
@@ -348,10 +388,10 @@ Section Move.
     {
       intros tin k (x&HEncX&Hk).
       destruct HEncX as (r1&->).
-      rewrite MoveToSymbol_TermTime_midtape; auto. now rewrite map_length. 
+      rewrite MoveToSymbol_TermTime_midtape; auto. now rewrite map_length.
     }
   Qed.
-  
+
   Lemma MoveLeft_Terminates :
     projT1 MoveLeft ↓ (fun tin k => exists x, tin[@Fin0] ≂ x /\ 8 + 4 * length (encode x : list sig) <= k).
   Proof.
@@ -360,245 +400,75 @@ Section Move.
     {
       intros tin k (x&HEncX&Hk).
       destruct HEncX as (r1&->).
-      rewrite MoveToSymbol_TermTime_midtape_l; auto. now rewrite map_length, rev_length. 
+      rewrite MoveToSymbol_L_TermTime_midtape; auto. now rewrite map_length, rev_length.
     }
   Qed.
 
 End Move.
 
 
-(* TODO: CopyValue *)
-
-
-(*
-
-Section Reset.
-  Variable (sig: finType) (X:Type) (cX: codeable sig X).
-
-  Definition Reset := Return (MoveToSymbol (fun (s: sig^+) => false)) tt;; Move _ L tt.
-
-  Definition Reset_Rel : Rel (tapes (sig^+) 1) (unit * tapes (sig^+) 1) :=
-    Mk_R_p (ignoreParam (fun tin tout => forall x:X, tin ≃ x -> tout ≂ x)).
-
-  Lemma Reset_WRealise : Reset ⊫ Reset_Rel.
-  Proof.
-    eapply WRealise_monotone.
-    { unfold Reset. repeat TM_Correct. }
-    { intros tin ((), tout) H. intros x HEncX. TMSimp. clear_trivial_eqs. clear H3.
-      destruct HEncX as (y&ys&rs&HECode&HEncX). rewrite HEncX.
-      pose proof MoveToSymbol_correct_toRight (inl START :: rs) (inr y) (map inr ys) as (HMove1&HMove2).
-      cbn in *. unfold finType_CS in *. (* rewrite <- HEncX, <- H2 in HMove1, HMove2. *)
-      destruct (rev _).
-      - apply (conj HMove2) in HMove1. eapply midtape_tape_local_l_cons_right in HMove1.
-        rewrite HMove1. repeat econstructor. all: admit.
-      - apply (conj HMove2) in HMove1. eapply midtape_tape_local_l_cons_right in HMove1.
-        rewrite HMove1. repeat econstructor. all: admit.
-    }
-  Admitted.
-
-End Reset.
-
-
-(* Copy a value from to an internal (right) tape *)
+(** Copy a value from to an internal (right) tape *)
 Section CopyValue.
   Variable (sig: finType) (X:Type) (encX: codeable sig X).
 
-  (** The tape "almost" contains the value x, but the pointer of the tape is right. *)
-  Definition tape_contains_rew (t: tape (sig^+)) x :=
-    exists (y : sig) (ys : list sig) (r1 : list (start + sig)),
-      encode x = (ys ++ [y] : list sig) /\ t = midtape (map inr ys ++ inl START :: r1) (inr y) nil.
-  Notation "t ≂ x" := (tape_contains_rew t x) (at level 70).
 
-  Lemma tape_contains_rew_isRight t x :
-    t ≂ x -> isRight t.
-  Proof. intros (y&ys&r1&HCode&->). repeat econstructor. Qed.
+  Definition CopyValue :=
+    Inject (MoveRight _) [|Fin0|];; CopySymbols_L (@isStart sig) id.
+
+  Definition CopyValue_Rel : Rel (tapes (sig^+) 2) (unit * tapes (sig^+) 2) :=
+    ignoreParam (
+        fun tin tout =>
+          forall x:X,
+            tin[@Fin0] ≃ x ->
+            isRight tin[@Fin1] ->
+            tout[@Fin0] ≃ x /\
+            tout[@Fin1] ≃ x
+      ).
 
 
-(** CopyValue := t0:Reset; CopySymbols_L (stop at the start symbol); 1-2: Move(R) *)
+  Lemma CopyValue_WRealise : CopyValue ⊫ CopyValue_Rel.
+  Proof.
+    eapply WRealise_monotone.
+    { unfold CopyValue. repeat TM_Correct. eapply MoveRight_WRealise with (X := X). }
+    {
+      intros tin ((), tout) H.
+      intros x HEncX HRight.
+      destruct HRight as (r1&r2&HRight).
+      TMSimp. clear H1.
+      apply H in HEncX. clear H. destruct HEncX as (r3&HEncX). rewrite HEncX in H0.
+      erewrite CopySymbols_L_correct_midtape in H0; eauto.
+      - inv H0. TMSimp. repeat econstructor; now rewrite map_rev, rev_involutive.
+      - intros ? (?&<-&?) % in_map_iff. reflexivity.
+    }
+  Qed.
 
+  (* TODO: Runtime *)
 
-  
+  Lemma CopyValue_Terminats :
+    projT1 CopyValue ↓ (fun tin k => exists x:X, tin[@Fin0] ≃ x /\ 25 + 12 * (length (encode x : list sig)) <= k).
+  Proof.
+    eapply TerminatesIn_monotone.
+    { unfold CopyValue. repeat TM_Correct.
+      - eapply MoveRight_WRealise.
+      - eapply MoveRight_Terminates. }
+    {
+      intros tin k (x&HEncX&Hk).
+      exists (8 + 4 * length (encode x : list sig)), (16 + 8 * length (encode x : list sig)). repeat split; cbn.
+      - omega.
+      - eauto.
+      - intros tmid () (H1&HInj). TMSimp.
+        apply H1 in HEncX as (r1&->).
+        rewrite CopySymbols_L_TermTime_midtape; eauto.
+        now rewrite map_length, rev_length.
+    }
+  Qed.
 
 End CopyValue.
 
 
-
 (*
-(* TODO *)
 
-Section Copy_code.
-  Variable sig : finType.
-  Variable X : Type.
-  Variable encX : codeable sig X.
-
-
-  Variable stop_X : sig -> bool.
-  Hypothesis stop_X_notInX : forall x : X, forall s : sig, List.In s (encode x) -> stop_X s = false.
-
-  Definition stop : (sig^+) -> bool :=
-    fun s => match s with
-          | inl _ => true
-          | inr x => stop_X x
-          end.
-
-  Lemma stop_notInX (x : X) (s : (sig^+)) :
-    List.In s (encode x) -> stop s = false.
-  Proof. cbn. intros (?&<-&?) % in_map_iff. cbn. eapply stop_X_notInX; eauto. Qed.
-
-
-  Definition MoveToSymbol_Code := Return (MoveToSymbol stop) tt.
- 
-  Definition MoveToSymbol_Code_Rel : Rel (tapes (sig^+) 1) (unit * tapes (sig^+) 1) :=
-    Mono.Mk_R_p (
-        ignoreParam (
-            fun tin tout =>
-              forall (x : X) r1 r2,
-                tape_encodes_l _ tin x r1 r2 ->
-                tout = midtape (rev (encode x) ++ inl START :: r1) (inl STOP) r2
-          )
-      ).
-
-
-  
-  Lemma MoveToSymbol_Code_WRealise :
-    MoveToSymbol_Code ⊫ MoveToSymbol_Code_Rel.
-  Proof.
-    eapply WRealise_monotone.
-    { unfold MoveToSymbol_Code. repeat TM_Correct. }
-    {
-      intros tin ((), tout). TMSimp. clear_trivial_eqs. clear H2.
-      destruct H0 as (HE1&HE2).
-      unfold finType_CS in *.
-      destruct (encode x) eqn:E1.
-      - eapply (MoveToSymbol_correct (stop := stop)) in HE2; eauto. unfold finType_CS in *. rewrite HE2.
-        cbn in *. rewrite HE1, E1. cbn. trivial.
-      - eapply (MoveToSymbol_correct (stop := stop)) in HE2; eauto. unfold finType_CS in *. rewrite HE2.
-        + cbn in *. rewrite HE1, E1. cbn. trivial.
-        + intros ? [-> | ?]; eapply (@stop_notInX x); unfold finType_CS in *; rewrite E1; eauto.
-    }
-  Qed.
-
-  Lemma MoveToSymbol_Code_Terminates :
-    projT1 MoveToSymbol_Code ↓
-           (fun tin k => exists x : X, tin[@Fin.F1] ≂ x /\ 4 + 4 * length (encode x) <= k).
-  Proof.
-    eapply TerminatesIn_monotone.
-    { unfold MoveToSymbol_Code. repeat TM_Correct. }
-    {
-      intros tin k. intros (x&HEncX&HTx).
-      destruct HEncX as (r1&r2&HE1&HE2).
-      pose proof MoveToSymbols_TermTime_local (stop := stop) HE2 ltac:(trivial).
-      rewrite <- HTx. progress unfold finType_CS in *. rewrite H.
-      eapply Nat.add_le_mono. omega. cbn. simpl_list. omega.
-    }
-  Qed.
-
-
-
-  Definition MoveToSymbol_Code_L := Return (MoveToSymbol_L stop) tt.
-
-  Definition MoveToSymbol_Code_L_Rel : Rel (tapes (sig^+) 1) (unit * tapes (sig^+) 1) :=
-    Mono.Mk_R_p (
-        ignoreParam (
-            fun tin tout =>
-              forall (x : X) r1 r2,
-                tape_encodes_r _ tin x r1 r2 ->
-                tout = midtape r1 (inl START) (encode x ++ inl STOP :: r2)
-          )
-      ).
-
-    
-  Lemma MoveToSymbol_Code_L_WRealise :
-    MoveToSymbol_Code_L ⊫ MoveToSymbol_Code_L_Rel.
-  Proof.
-    eapply WRealise_monotone.
-    { unfold MoveToSymbol_Code_L. repeat TM_Correct. }
-    {
-      intros tin ((), tout). TMSimp. clear_trivial_eqs. clear H2.
-      destruct H0 as (HE1&HE2).
-      unfold finType_CS in *.
-      destruct (encode x) eqn:E1.
-      - eapply (MoveToSymbol_L_correct (stop := stop)) in HE2; eauto.
-        + unfold finType_CS in *. rewrite HE2. cbn in *. rewrite E1, HE1. cbn. trivial.
-        + cbn. auto.
-      - eapply (MoveToSymbol_L_correct (stop := stop)) in HE2; eauto.
-        + unfold finType_CS in *. rewrite HE2. cbn in *. rewrite E1, HE1. cbn. simpl_list. cbn. trivial.
-        + intros ? [ -> | ? ] % in_rev; eapply (@stop_notInX x); unfold finType_CS; rewrite E1; auto.
-    }
-  Qed.
-
-  Lemma MoveToSymbol_Code_L_Terminates :
-    projT1 MoveToSymbol_Code_L ↓
-           (fun tin k => exists x : X, tape_encodes' _ tin[@Fin.F1] x /\ 4 + 4 * length (encode x) <= k).
-  Proof.
-    eapply TerminatesIn_monotone.
-    { unfold MoveToSymbol_Code_L. repeat TM_Correct. }
-    {
-      intros tin k. intros (x&HEncX&HTx).
-      destruct HEncX as (r1&r2&HE1&HE2).
-      pose proof MoveToSymbols_TermTime_local_l (stop := stop) HE2 ltac:(trivial).
-      rewrite <- HTx. progress unfold finType_CS in *. rewrite H.
-      eapply Nat.add_le_mono. omega. cbn. simpl_list. omega.
-    }
-  Qed.
-  
-
-
-  (** Copy *)
-
-  Definition CopySymbols_Code := CopySymbols stop id.
-
-  Definition CopySymbols_Code_Rel : Rel (tapes (sig^+) 2) (unit * tapes (sig^+) 2) :=
-    ignoreParam (
-        fun tin tout =>
-          forall x r1 r2,
-            tape_encodes_l _ tin[@Fin0] x r1 r2 ->
-            tout[@Fin0] = midtape (rev (encode x) ++ inl START :: r1) (inl STOP) r2 /\
-            tout[@Fin1] = midtape (rev (encode x) ++ left tin[@Fin1]) (inl STOP) (skipn (|encode x|) (right tin[@Fin1]))
-      ).
-
-  Lemma CopySymbols_Code_WRealise :
-    CopySymbols_Code ⊫ CopySymbols_Code_Rel.
-  Proof.
-    eapply WRealise_monotone.
-    { unfold CopySymbols_Code. repeat TM_Correct. }
-    {
-      intros tin ((), tout) H. intros x r1 r2 HEncX. cbn in H.
-      destruct HEncX as (HE1&HE2).
-      destruct (encode x : list sig) eqn:E1.
-      - unshelve epose proof CopySymbols_pair_correct (stop := stop) (tltr := (tin[@Fin0], tin[@Fin1])) as L. cbn in L.
-        specialize L with (3 := HE2). cbn in L. rewrite E1 in L. cbn in L. do 2 spec_assert L by eauto.
-        unfold finType_CS in *. rewrite L in H. injection H as H1 H2.
-        rewrite H1, H2. cbn in *. rewrite E1, HE1. cbn. auto.
-      - unshelve epose proof CopySymbols_pair_correct (stop := stop) (tltr := (tin[@Fin0], tin[@Fin1])) as L. cbn in L.
-        specialize L with (3 := HE2). cbn in L. rewrite E1 in L. cbn in L.
-        spec_assert L.
-        { intros ? [<- | ?]; eapply (@stop_notInX x); cbn; rewrite E1; cbn; eauto. }
-        spec_assert L by auto.
-        unfold finType_CS in *. rewrite L in H. injection H as H1 H2.
-        rewrite H1, H2. cbn in *. rewrite E1, HE1. cbn.
-        rewrite map_length. auto.
-    }
-  Qed.
-
-  Lemma CopySymbols_Code_Terminates :
-    projT1 CopySymbols_Code ↓ (fun tin k => exists x : X, tin[@Fin.F1] ≂ x /\ 8 + 8 * length (encode x) <= k).
-  Proof.
-    eapply TerminatesIn_monotone.
-    { unfold CopySymbols_Code. repeat TM_Correct. }
-    {
-      intros tin k (x&HencX&Hk). rewrite <- Hk.
-      destruct HencX as (r1&r2&HEnc1&HEnc2).
-      epose proof CopySymbols_TermTime_local (stop := stop) HEnc2 ltac:(trivial) as L.
-      rewrite L.
-      eapply Nat.add_le_mono. omega. cbn. simpl_list. omega.
-    }
-  Qed.
-  
-  (* TODO: Gespiegelte Variante *)
-                 
-End Copy_code.
-
+(* TODO: Arguments *)
 
 Arguments MoveToSymbol_Code : simpl never.
 Arguments MoveToSymbol_Code_L : simpl never.
@@ -608,448 +478,6 @@ Arguments MoveToSymbol_Code_Rel { sig X encX } x y /.
 Arguments MoveToSymbol_Code_L_Rel { sig X encX } x y /.
 Arguments CopySymbols_Code_Rel { sig X encX } x y /.
 
-
-
-
-Section MoveToOtherSideOfTheEncoding.
-
-  Variable sig : finType.
-  Variable X : Type.
-  Variable encX : codeable sig X.
-
-  Definition dontStop : sig -> bool := fun _ => false.
-
-  Definition MoveToRightCode :=
-    MoveToSymbol_Code dontStop;;
-    Move _ L tt.
-
-  Definition MoveToRightCode_Rel : Rel (tapes (sig^+) 1) (unit * tapes (sig^+) 1) :=
-    Mk_R_p (
-        ignoreParam (
-        fun tin tout =>
-          forall (x : X) r1 r2,
-            tape_encodes_l _ tin x r1 r2 ->
-            tape_encodes_r _ tout x r1 r2
-          )
-      ).
-
-  Lemma MoveToRightCode_WRealse :
-    MoveToRightCode ⊫ MoveToRightCode_Rel.
-  Proof.
-    eapply WRealise_monotone.
-    { unfold MoveToRightCode. repeat TM_Correct. eapply MoveToSymbol_Code_WRealise. eauto. }
-    {
-      intros tin ((), tout) H. TMSimp. clear_trivial_eqs.
-      specialize (H _ _ _ H0) as ->. cbn.
-      hnf. hnf in H0. destruct H0 as (HE1&HE2).
-      simpl_tape; auto.
-    }
-  Qed.
-
-  Lemma MoveToRightCode_Terminates :
-    projT1 MoveToRightCode ↓
-           (fun tin k => exists x : X, tin[@Fin.F1] ≂ x /\ 6 + 4 * length (encode x) <= k).
-  Proof.
-    eapply TerminatesIn_monotone.
-    {
-      unfold MoveToRightCode. repeat TM_Correct. 
-      - apply MoveToSymbol_Code_WRealise; auto.
-      - apply MoveToSymbol_Code_Terminates; auto.
-    }
-    {
-      intros tin k (x&HEncX&Hk).
-      exists (4 + 4 * length (encode x)), 1. repeat split.
-      - omega.
-      - exists x. split. auto. omega.
-      - auto.
-    }
-  Qed.
-  
-    
-
-  Definition MoveToLeftCode :=
-    MoveToSymbol_Code_L dontStop;;
-    Move _ R tt.
-
-  Definition MoveToLeftCode_Rel : Rel (tapes (sig^+) 1) (unit * tapes (sig^+) 1) :=
-    Mk_R_p (
-        ignoreParam (
-        fun tin tout =>
-          forall (x : X) r1 r2,
-            tape_encodes_r _ tin x r1 r2 ->
-            tape_encodes_l _ tout x r1 r2
-          )
-      ).
-
-  Lemma MoveToLeftCode_WRealse :
-    MoveToLeftCode ⊫ MoveToLeftCode_Rel.
-  Proof.
-    eapply WRealise_monotone.
-    { unfold MoveToLeftCode. repeat TM_Correct. eapply MoveToSymbol_Code_L_WRealise. eauto. }
-    {
-      intros tin ((), tout) H. TMSimp. clear_trivial_eqs.
-      specialize (H _ _ _ H0) as ->. cbn.
-      hnf. hnf in H0. destruct H0 as (HE1&HE2).
-      simpl_tape; auto.
-    }
-  Qed.
-
-  
-  Lemma MoveToLeftCode_Terminates :
-    projT1 MoveToLeftCode ↓
-           (fun tin k => exists x : X, tape_encodes' _ tin[@Fin.F1] x /\ 6 + 4 * length (encode x) <= k).
-  Proof.
-    eapply TerminatesIn_monotone.
-    {
-      unfold MoveToLeftCode. repeat TM_Correct. 
-      - apply MoveToSymbol_Code_L_WRealise; auto.
-      - apply MoveToSymbol_Code_L_Terminates.
-    }
-    {
-      intros tin k (x&HEncX&Hk).
-      exists (4 + 4 * length (encode x)), 1. repeat split.
-      - omega.
-      - exists x. split. auto. omega.
-      - auto.
-    }
-  Qed.
-
-
-
-  (** Copy values from one tape to another tape *)
-
-  Definition CopyValue :=
-    Inject (WriteMove (Some (inl START), R) tt) [|Fin.FS Fin.F1|];;
-    CopySymbols_Code dontStop;;
-    MovePar _ L L tt.
-
-  Definition CopyValue_Rel : Rel (tapes (sig^+) 2) (unit * tapes (sig^+) 2) :=
-    ignoreParam (
-        fun tin tout =>
-          forall (x : X) r1 r2,
-            tin [@Fin0] ≂[r1; r2] x ->
-            tout[@Fin0] ≃[r1; r2] x /\
-            tout[@Fin1] ≃[left tin[@Fin1]; skipn (S (|encode x|)) (right tin[@Fin1])] x
-      ).
-
-  Lemma CopyValue_WRealise :
-    CopyValue ⊫ CopyValue_Rel.
-  Proof.
-    eapply WRealise_monotone.
-    { unfold CopyValue. repeat TM_Correct. eapply CopySymbols_Code_WRealise; auto. }
-    {
-      intros tin ((), tout) H. intros x r1 r2 HEncX. TMSimp; clear_trivial_eqs. clear H4 H5.
-      clear H1 H2. simpl_tape in H0.
-      specialize (H0 _ _ _ HEncX) as (L1&L2). rewrite L1, L2. clear L1 L2.
-      destruct HEncX as (HE1&HE2). split.
-      - hnf. split.
-        + cbn. simpl_tape. auto.
-        + cbn. simpl_tape. auto.
-      - hnf. split.
-        + cbn. simpl_tape. f_equal. destruct (right tin[@Fin1]); cbn; auto using skipn_nil.
-        + erewrite tape_local_l_move_left; eauto. eapply tape_local_l_cons_iff; cbn; eauto.
-    }
-  Qed.
-
-  Lemma CopyValue_Terminates :
-    projT1 CopyValue ↓ (fun tin k => exists x, tin[@Fin.F1] ≂ x /\ 14 + 8 * length (encode x) <= k).
-  Proof.
-    eapply TerminatesIn_monotone.
-    {
-      unfold CopyValue. repeat TM_Correct. 
-      - apply CopySymbols_Code_WRealise; auto.
-      - apply CopySymbols_Code_Terminates.
-    }
-    {
-      intros tin k. intros (x&HEnc&Hk).
-      exists 1, (12 + 8 * length (encode x)). repeat split.
-      - omega.
-      - hnf. omega.
-      - intros tout () (H1&H2). hnf in H1, H2. simpl_not_in.
-        exists (8 + 8 * length (encode x)), 3. repeat split.
-        + omega.
-        + exists x. repeat split; eauto. unfold finType_CS in *. rewrite <- H2. auto.
-        + intros ? ? ?. omega.
-    }
-  Qed.
-
-
-  Definition CopyValue' :=
-    CopyValue;; (* 14 + 8 * length (encode x) *)
-    Inject MoveToLeftCode [|Fin.F1|];; (* 6 + 4 * length (encode x) *)
-    Inject MoveToLeftCode [|Fin.FS Fin.F1|]. (* 6 + 4 * length (encode x) *)
-  (* 28 + 16 * length (encode x) *)
-
-  Definition CopyValue'_Rel : Rel (tapes (sig^+) 2) (unit * tapes (sig^+) 2) :=
-    ignoreParam (
-        fun tin tout =>
-          forall (x : X) r1 r2,
-            tin [@Fin0] ≂[r1; r2] x ->
-            tout[@Fin0] = tin[@Fin0] /\
-            tout[@Fin1] ≂[left tin[@Fin1]; skipn (S (|encode x|)) (right tin[@Fin1])] x
-      ).
-
-  Lemma CopyValue'_WRealise :
-    CopyValue' ⊫ CopyValue'_Rel.
-  Proof.
-    eapply WRealise_monotone.
-    {
-      unfold CopyValue'. repeat TM_Correct.
-      - eapply CopyValue_WRealise.
-      - eapply MoveToLeftCode_WRealse.
-      - eapply MoveToLeftCode_WRealse.
-    }
-    {
-      intros tin ((), yout) H. intros x r1 r2 HEncX. TMSimp.
-      unfold finType_CS in *. clear H3.
-      specialize (H _ _ _ HEncX) as (L1&L2).
-      specialize (H0 _ _ _ L1).
-      specialize (H1 _ _ _ L2).
-      split.
-      - eapply tape_encodes_l_injective; eauto.
-      - hnf; eauto.
-    }
-  Qed.
-  
-  Lemma CopyValue'_Terminates :
-    projT1 CopyValue' ↓ (fun tin k => exists x, tin[@Fin.F1] ≂ x /\ 28 + 16 * length (encode x) <= k).
-  Proof.
-    eapply TerminatesIn_monotone.
-    {
-      unfold CopyValue'. repeat TM_Correct.
-      - eapply CopyValue_WRealise.
-      - eapply CopyValue_Terminates.
-      - eapply MoveToLeftCode_WRealse.
-      - eapply MoveToLeftCode_Terminates.
-      - eapply MoveToLeftCode_Terminates.
-    }
-    {
-      intros tin k (x&HEncX&Hk).
-      exists (14 + 8 * length (encode x)), (13 + 8 * length (encode x)). repeat split.
-      - omega.
-      - eauto.
-      - intros tout () H.
-        destruct HEncX as (r1&r2&HE).
-        hnf in H. specialize (H _ _ _ HE) as (L1&L2).
-        exists (6 + 4 * length (encode x)), (6 + 4 * length (encode x)). repeat split.
-        + omega.
-        + hnf. exists x. split. cbn. do 2 eexists. eauto. omega.
-        + intros tout' () (H1&H2).
-          hnf in H1, H2. simpl_not_in. cbn in H1.
-          specialize (H1 _ _ _ L1). hnf.
-          exists x. split. cbn. rewrite <- H2. hnf; eauto. omega.
-    }
-  Qed.
-  
-
-End MoveToOtherSideOfTheEncoding.
-
-Arguments MoveToRightCode : simpl never.
-Arguments MoveToLeftCode : simpl never.
-Arguments CopyValue : simpl never.
-Arguments CopyValue' : simpl never.
-
-
-Section RestoreValue.
-
-  Variable sig : finType.
-  Variable (X : Type) (codX : codeable sig X).
-
-  Definition MoveToLeft_Rel : Rel (tapes (sig^+) 1) (unit * tapes (sig^+) 1) :=
-    Mk_R_p (
-        ignoreParam (
-            fun tin tout =>
-              forall x r1 r2,
-                tin ≂[r1; r2] x ->
-                left tout = nil /\
-                tape_local tout = rev r1 ++ inl START :: encode x ++ inl STOP :: r2
-          )
-      ).
-
-  Definition MoveToLeft :=
-    MoveToSymbol_L (fun _ : (sig^+) => false);; (* 4 + 4 * (S (S (|r1| + |encode x|))) *)
-    Move _ R tt. (* 1 *)
-  (* 14 + 4 * (|r1| + |encode x|) *)
-
-  Lemma MoveToLeft_WRealise : MoveToLeft ⊫ MoveToLeft_Rel.
-  Proof.
-    eapply WRealise_monotone.
-    { unfold MoveToLeft. repeat TM_Correct. }
-    {
-      intros tin ((), tout) H. intros x r1 r2 HEncX.
-      TMSimp. clear H H2 H0 H1.
-      destruct HEncX as (HE1 & HE2).
-      destruct (encode x : list sig) eqn:E1; cbn in *; rewrite E1 in *; cbn in *.
-      - apply midtape_tape_local_cons in HE2. unfold finType_CS in *. rewrite HE1 in HE2. rewrite HE2.
-        pose proof MoveToSymbol_L_correct_toLeft (inl START :: r1) (inl STOP) r2 as (L1&L2).
-        unfold finType_CS in *. cbn in *. rewrite L1, L2. split; auto. simpl_list. cbn. simpl_list. cbn. auto.
-      - apply midtape_tape_local_cons in HE2. unfold finType_CS in *. rewrite HE1 in HE2. rewrite HE2.
-        pose proof MoveToSymbol_L_correct_toLeft (inl START :: r1) (inr e) (map inr l ++ inl STOP :: r2) as (L1&L2).
-        cbn in L1, L2. rewrite <- app_assoc in L2. cbn in *.
-        destruct (tape_move_right _) eqn:E2; cbn in *; subst; try now apply app_cons_not_nil in L2. eauto.
-    }
-  Qed.
-
-  Definition MoveToLeft_Rel' : Rel (tapes (sig^+) 1) (unit * tapes (sig^+) 1) :=
-    Mk_R_p (
-        ignoreParam (
-            fun tin tout =>
-              forall x,
-                tin ≂ x ->
-                isLeft tout
-          )
-      ).
-
-  Lemma MoveToLeft_WRealise' : MoveToLeft ⊫ MoveToLeft_Rel'.
-  Proof.
-    eapply WRealise_monotone.
-    { apply MoveToLeft_WRealise. }
-    {
-      intros tin ((), tout) H. cbn in *. intros x (r1&r2&HEncX).
-      specialize (H _ _ _ HEncX) as (H1&H2).
-      hnf. destruct (rev r1) eqn:E1; cbn in *; rewrite E1 in H2; cbn in *.
-      - apply (conj H1) in H2. apply midtape_tape_local_cons_left in H2 as ->. eauto.
-      - apply (conj H1) in H2. apply midtape_tape_local_cons_left in H2 as ->. eauto.
-    }
-  Qed.
-  
-
-  Lemma MoveToLeft_Terminates :
-    projT1 MoveToLeft ↓ (fun tin i => exists x r1 r2, tin[@Fin0] ≂[r1;r2] x /\ 14 + 4 * (|r1| + |encode x : list sig|) <= i).
-  Proof.
-    eapply TerminatesIn_monotone.
-    { unfold MoveToLeft. repeat TM_Correct. }
-    {
-      intros tin i (x&r1&r2&HEnc&Hi).
-      exists (12 + 4 * (|r1| + |encode x|)), 1. repeat split.
-      - omega.
-      - destruct HEnc as (HE1&HE2).
-        destruct (encode x : list sig) eqn:E1; cbn -[plus mult] in *; rewrite E1 in *; cbn -[plus mult] in *.
-        + apply tape_local_cons_iff in HE2 as (HE2&HE3).
-          apply (conj HE2) in HE1. apply tape_local_l_cons_iff in HE1.
-          pose proof MoveToSymbol_L_TermTime_dontstop tin[@Fin0] as L.
-          rewrite HE1 in L. cbn -[plus mult] in *. omega.
-        + apply tape_local_cons_iff in HE2 as (HE2&HE3).
-          apply (conj HE2) in HE1. apply tape_local_l_cons_iff in HE1.
-          pose proof MoveToSymbol_L_TermTime_dontstop tin[@Fin0] as L.
-          rewrite HE1 in L. cbn -[plus mult] in *. omega.
-      - intros _ _ _. omega.
-    }
-  Qed.
-
-
-  (* Restore the saved value from tape 1 to tape 0 *)
-  Definition RestoreValue : { M : mTM (sig^+) 2 & states M -> unit } :=
-    Inject MoveToLeft [|Fin0|];; (* 14 + 4 * (|s1| + |encode x1|) *)
-    Inject (CopyValue' _) [|Fin1; Fin0|];; (* 28 + 16 * |encode x2| *)
-    Inject MoveToLeft [|Fin1|]. (* 14 + 4 * (|nil| + |encode x2|) *)
-  (* 43 + 20 * (|encode x2|) *)
-  (* 58 + 4 * |s1| + 4 * (|encode x1|) + 20 * (|encode x2|) *)
-
-  Definition RestoreValue_Rel : Rel (tapes (sig^+) 2) (unit * tapes (sig^+) 2) :=
-    ignoreParam (
-        fun tin tout =>
-          forall x1 x2 r1 r2 r3,
-            (* x2 is the saved value, x1 is the value that is currently on the working tape *)
-            tin [@Fin0] ≂[r1; r2] x1 ->
-            tin [@Fin1] ≂[nil; r3] x2 ->
-            tout[@Fin0] ≂[nil; skipn (S (S (|encode x2|))) (rev r1 ++ inl START :: encode x1 ++ inl STOP :: r2)] x2 /\
-            tout[@Fin1] = midtape nil (inl START) (encode x2 ++ inl STOP :: r3)
-      ).
-
-  Lemma RestoreValue_WRealise : RestoreValue ⊫ RestoreValue_Rel.
-  Proof.
-    eapply WRealise_monotone.
-    {
-      unfold RestoreValue. repeat TM_Correct.
-      - eapply MoveToLeft_WRealise.
-      - eapply CopyValue'_WRealise.
-      - eapply MoveToLeft_WRealise.
-    }
-    {
-      intros tin ((), tout) H. intros x1 x2 r1 r2 r3 HEncX1 HEncX2. TMSimp.
-      specialize (H _ _ _ HEncX1) as (H&H').
-      specialize (H0 _ _ _ HEncX2) as (H0&H0'). rewrite H0 in *. clear H0.
-      specialize (H2 _ _ _ HEncX2) as (H2&H2').
-      rewrite H in *.
-      cbn in *.
-      destruct HEncX2 as (HEncX21&HEncX22).
-      destruct H0' as (HEncX2out1&HEncX2out2).
-      split.
-      - split. auto. unfold finType_CS in *. rewrite HEncX2out2. cbn. f_equal. f_equal.
-        unfold finType_CS in *.
-        destruct (rev r1) eqn:E1; cbn in *.
-        + apply tape_local_cons_iff in H' as (H'&H''). unfold finType_CS in *. cbn in *. rewrite H''. auto.
-        + apply tape_local_cons_iff in H' as (H'&H''). unfold finType_CS in *. cbn in *. rewrite H''. auto.
-      - apply midtape_tape_local_cons in H2' as ->. f_equal. auto.
-    }
-  Qed.
-
-
-  Definition RestoreValue_Rel_size : Rel (tapes (sig^+) 2) (unit * tapes (sig^+) 2) :=
-    ignoreParam (
-        fun tin tout =>
-          forall x1 x2 s1 s2 s3,
-            tin [@Fin0] ≂{s1;s2} x1 ->
-            tin [@Fin1] ≂{0;s3} x2 ->
-            tout[@Fin0] ≂{0; (s1 + |encode x1| + s2) - (|encode x2|)} x2 /\
-            isLeft_size tout[@Fin1] (S (|encode x2|) + s3)
-      ).
-
-  Lemma RestoreValue_WRealise_size : RestoreValue ⊫ RestoreValue_Rel_size.
-  Proof.
-    eapply WRealise_monotone. eapply RestoreValue_WRealise.
-    {
-      intros tin ((), tout) H. intros x1 x2 s1 s2 s3 HEncX1 HEncX2. TMSimp.
-      destruct HEncX1 as (r1&r2&Hr1&Hr2&HEncX1). destruct HEncX2 as (r1'&r2'&Hr1'&Hr2'&HEncX2).
-      destruct r1'; cbn in *; try omega. clear Hr1'. unfold finType_CS in *.
-      specialize (H _ _ _ _ _ HEncX1 HEncX2) as (H1&H2).
-      split.
-      - hnf. exists nil. eexists. split. cbn. omega. split; swap 1 2. eauto.
-        rewrite skipn_length, app_length, rev_length. cbn. rewrite app_length, map_length. cbn. omega.
-      - hnf. eexists. eexists. split; swap 1 2. eauto.
-        rewrite app_length, map_length. cbn. omega.
-    }
-  Qed.
-
-
-  Lemma RestoreValue_Terminates :
-    projT1 RestoreValue ↓
-           (fun tin i =>
-              exists x1 x2 s1 s2 s3,
-                tin [@Fin0] ≂{s1; s2} x1 /\
-                tin [@Fin1] ≂{0;  s3} x2 /\
-                58 + 4 * s1 + 4 * (|encode x1|) + 20 * (|encode x2|) <= i).
-  Proof.
-    eapply TerminatesIn_monotone.
-    {
-      unfold RestoreValue. repeat TM_Correct.
-      - eapply MoveToLeft_WRealise.
-      - eapply MoveToLeft_Terminates.
-      - eapply CopyValue'_WRealise.
-      - eapply CopyValue'_Terminates.
-      - eapply MoveToLeft_Terminates.
-    }
-    {
-      intros tin i. intros (x&y&s1&s2&s3&HEncX&HEncY&Hi).
-      destruct HEncX as (r1&r2&Hr1&Hr2&HEncX). destruct HEncY as (r1'&r2'&Hr1'&Hr2'&HEncY).
-      destruct r1'; cbn -[plus mult] in *; try omega. clear Hr1'.
-      exists (14 + 4 * s1 + 4 * |encode x|), (43 + 20 * (|encode y|)). repeat split.
-      - omega.
-      - cbn -[plus mult]. do 3 eexists. split. eauto. cbn [length]. omega.
-      - intros tmid1 () (H1&H2). simpl_not_in. rewrite H2 in *. clear H2.
-        specialize (H1 _ _ _ ltac:(eauto)) as (H1&H2). cbn -[plus mult] in *.
-        exists (28 + 16 * |encode y|), (14 + 4 * |encode y|). repeat split.
-        + omega.
-        + eexists. split. hnf. eauto. omega.
-        + intros tmid2 () (H3&H4). clear H4.
-          specialize (H3 _ _ _ ltac:(hnf; eauto)) as (H4&H5). unfold finType_CS in *. rewrite H4.
-          do 3 eexists. split. hnf; eauto. cbn [length]. omega.
-    }
-  Qed.
-
-End RestoreValue.
-
 Arguments MoveToLeft : simpl never.
 Arguments RestoreValue : simpl never.
 
@@ -1057,8 +485,6 @@ Arguments MoveToLeft_Rel { sig X } (codX) x y /.
 Arguments RestoreValue_Rel { sig X } (codX) x y /.
 Arguments RestoreValue_Rel_size { sig X } (codX) x y /.
 
-
-(* todo: Arguments, smpl, etc. *)
 
 
 (*
@@ -1072,5 +498,4 @@ Ltac smpl_TM_CopyMoveCode :=
 Smpl Add smpl_TM_CopyMoveCode : TM_Correct.
 *)
 
-*)
 *)
